src/PlutusIR/Semantics/Static/normaliser/STLC_norm_completeness.v
@@ -1,29 +1,106 @@
-From PlutusCert Require Import STLC_named STLC_normalisation SN_STLC_named STLC_named_typing.
+From PlutusCert Require Import STLC_named STLC_normalisation SN_STLC_named STLC_named_typing util.
 Require Import Coq.Lists.List.
 Import ListNotations.
 
-(* sound: if function, then relation*)
-(* complete: if relation, then function*)
+Require Import Coq.Program.Equality.
 
-(* Lemma strong_normalization_SN :
-  forall E s T (H : SN_STLC_named.has_type E s T), strong_normalization H = SN s.
+(* Used to do induction over the size of SN proofs *)
+Fixpoint mysn_size {t : term} (HSN : MySN t) : nat :=
+  match HSN with
+  | SNI0 _ => 0
+  | SNI' (existT _ t' (_, HSN')) => 1 + mysn_size HSN'
+  end.
+
+Lemma mysn_size_helper {t : term} (HSN : MySN t) :
+  forall f, @mysn_size t (SNI' f) <> 0.
 Proof.
-  (* This requires proving equivalence, likely with the definition of `strong_normalization`. *)
-Admitted. *)
+  intros f.
+  simpl.
+  destruct f as [t' p].
+  destruct p as [_ HSN'].
+  intros Hcontra.
+  inversion Hcontra.
+Qed.
 
-Lemma uhm t t' :
-  step_d_f t = t' -> True.
+Lemma norm_lam tb x T (snt : (MySN (tmlam x T tb))) (sntb : MySN tb):
+  @normalizer' (tmlam x T tb) snt = tmlam x T (@normalizer' tb sntb).
 Proof.
   intros.
-  destruct (step_d_f t) eqn:Heq.
-Admitted.
+  remember (mysn_size snt) as n.
+  generalize dependent tb.
+  dependent induction n.
+  - intros tb snt sntb Hsize.
+    remember snt as snt_copy.
+    clear Heqsnt_copy.
+    destruct snt_copy.
+    + (* no step for the outer lambda, so we should also get: no step for the inner lambda *)
+      induction sntb.
+      * simpl.
+        reflexivity.
+      * exfalso.
+        destruct s as [t' [Hstept' HSNt'] ].
+        clear Hsize.
+        inversion e.
+        unfold bind in H0.
+        assert (step_d_f tb = None) by destruct_match.
 
-Lemma x :
-  normalizer'' 
-Admitted.
+        rewrite Hstept' in H.
+        inversion H.
+    + exfalso.
+      inversion Hsize.
+      simpl in H0.
+      destruct H0.
+      assert (mysn_size (SNI' (t := tmlam x T tb) s) <> 0).
+      {
+        apply mysn_size_helper.
+        assumption.
+      }
+      rewrite <- Hsize in H.
+      contradiction.    
+  - induction sntb.
+    + intros Hsize.
+      induction snt.
+      * simpl. reflexivity.
+      * exfalso.
+        destruct s as [t' [Hstept' HSNt'] ].
+        clear Hsize.
+        inversion Hstept'.
+        unfold bind in H0.
+        assert (step_d_f tb <> None) by destruct_match.
+        (* contradiction: body does not step, while lambda does *)
+        contradiction.
+    + destruct snt.
+      * exfalso.
+        destruct s as [t' [Hstept' HSNt'] ].
+        inversion e.
+        unfold bind in H0.
+        destruct_match.
+      * 
+        
+        destruct s as [tb' [Hsteptb' HSNtb'] ].
+        destruct s0 as [t' [Hstept' HSNt'] ].
 
-Theorem norm_complete_mysn Δ K (t tn : term) (Hwt : SN_STLC_named.has_type Δ t K):
-  normalise t tn -> @normalizerMySN t Δ K Hwt = tn.
+        simpl.
+        assert (tmlam x T tb' = t').
+        {
+          inversion Hstept'.
+          unfold bind in H0.
+          destruct_match.
+          inversion H0.
+          inversion Hsteptb'.
+          reflexivity.
+        }
+        subst.
+        simpl.
+        specialize IHn with (tb := tb') (snt := HSNt') (sntb := HSNtb').
+        intros.
+        inversion Heqn.
+        specialize (IHn H0).
+        assumption.
+Qed.
+
+Theorem norm_complete Δ K (t tn : term) (Hwt : SN_STLC_named.has_type Δ t K):
+  normalise t tn -> @normalizer t Δ K Hwt = tn.
 Proof.
   intros HnormR.
   generalize dependent Δ.
@@ -34,111 +111,119 @@ Proof.
     specialize (IHHnormR1 (tp_arrow K1 K') Δ H2).
     specialize (IHHnormR3 (tp_arrow K1 K') Δ).
     admit.
-  - admit.
+  - inversion Hwt; subst.
+    specialize (IHHnormR2 K1 Δ H5).
+    specialize (IHHnormR1 (tp_arrow K1 K') Δ H3).
+
+    unfold normalizer.
+    unfold normalizer in IHHnormR1.
+    unfold normalizer in IHHnormR2.
+
+    (* Neutral T1n*)
+    subst.
+
+    destruct (strong_normalization_mysn H3).
+    + (* Case: Value $ T1*)
+      simpl.
+      
+      destruct (strong_normalization_mysn H5).
+      * (* Case Value T1 && Value T2 *)
+        simpl.
+        
+        destruct (strong_normalization_mysn Hwt).
+        -- (* Correct case: Value $ (tmapp T1 T2)*)
+           simpl. reflexivity.
+        -- (* Contradiction, T1 T2 no step, so app neither*)
+           exfalso.
+           destruct s as [t' [HstepT HSNt'] ].
+           inversion HstepT.
+
+           assert (is_normal T1 = true) by admit. (* should be clear from no step *)
+           rewrite H0 in H1.
+           assert (is_normal T2 = true) by admit.
+           rewrite H2 in H1.
+           simpl in H.
+           (* From H1 it follows that T1 must be of shape tmlam,
+            contradiction, because of H: T1 neutral*)
+           admit.
+          
+
+
+      * (* Case: Value T1 && Step T2 T2n *)
+        destruct (strong_normalization_mysn Hwt).
+        -- (* Contradiction: T2 steps, but tmapp not*)
+           exfalso.
+           inversion e0.
+           assert (is_normal T1 = true) by admit. 
+           rewrite H0 in H1.
+           assert (is_normal T2 = false) by admit.
+           rewrite H2 in H1.
+           unfold bind in H1.
+           (* H1 now says step_d_f T2 must be None, but s says it is Some*)
+           admit.
+        -- (* Correct case: T2 steps and app also steps *)           
+            destruct s as [t' [Hstept' HSNt'] ].
+            destruct s0 as [t'' [Hstept'' HSNt''] ].
+            simpl.
+            simpl in HnormR2.
+            simpl in HnormR1.
+            (* Not sure yet how to do this. 
+              Probably first get: t'' = tmapp T1 t', and then same as tmlam case
+            *)
+            admit.
+    + (* Case: step $ T1*)
+  
+    admit.
   - inversion Hwt; subst.
     specialize (IHHnormR K2 ((bX, K)::Δ) H4).
-    unfold normalizerMySN.
-    destruct (strong_normalization_mysn Hwt).
-    + unfold normalizer''.
-      unfold normalizerMySN in IHHnormR.
-      destruct (strong_normalization_mysn H4).
-      * unfold normalizer'' in IHHnormR. subst. reflexivity.
-      * (* Should yield a contradiction. 
-        If step_d_f T0 = Some t', then step_d_f (tmlam bX K T0) = Some (tmlam bX K t').
-
-
-        *)
-        inversion e.
+    
+    unfold normalizer; destruct (strong_normalization_mysn Hwt);
+    unfold normalizer';
+    unfold normalizer in IHHnormR; destruct (strong_normalization_mysn H4);
+    unfold normalizer' in IHHnormR.
+    + (* Already value*)
+      subst. reflexivity.
+    + exfalso. 
+      (* Contradiction: lambda no step, while body does. *)
+      inversion e.
+      unfold bind in H0.
+      destruct s as [t' [HstepT0' HSNt'] ].
+      destruct_match.  
+    + exfalso.
+      (* Contradiction: body does not step, while lambda does *)
+      destruct s as [t' [HstepT HSNt'] ]. 
+      inversion HstepT.
+      unfold bind in H0.
+      destruct_match.
+    + (* Body and whole lambda step *)
+      fold normalizer'.
+      destruct s as [t [Hstept HSNt] ].
+      destruct s0 as [tb [Hsteptb HSNtb] ].
+      fold normalizer' in IHHnormR.
+      assert (t = tmlam bX K tb).
+      {
+        inversion Hstept.
         unfold bind in H0.
-        assert (step_d_f T0 = None) by admit.
-        destruct s as [t' [HstepT0' HSNt'] ].
-        rewrite HstepT0' in H.
-        inversion H.      
-    + destruct s as [t' [HstepT HSNt'] ]. 
-      unfold normalizerMySN in IHHnormR.
-      destruct (strong_normalization_mysn H4) in IHHnormR.
-      * inversion HstepT.
-        unfold bind in H0.
-        assert (step_d_f T0 <> None) by admit. (* Follows from the match*)
-        contradiction.
-      * destruct s as [t'0 [HstepT0 HSNt'0] ].
-        (* unfold normalizer'' in IHHnormR. *)
-        unfold normalizer''.
-        destruct HSNt'.
-        inversion IHHnormR.
-        (* assert (t' = tmlam bX K t'0) by admit. *)
+        destruct_match.
+        inversion Hsteptb.
+        inversion H0.
         subst.
-        
-        f_equal.
-        subst.
-        admit.
-        admit.
-  
-  - unfold normalizerMySN.
+        reflexivity.
+      }
+      subst.
+      eapply norm_lam.
+  - unfold normalizer.
     destruct (strong_normalization_mysn Hwt).
-    unfold normalizer''.
+    unfold normalizer'.
     reflexivity.
-
-Theorem norm_complete Δ K (t tn : term) (Hwt : SN_STLC_named.has_type Δ t K) :
-    normalise t tn -> @normalizer t Δ K Hwt = tn.
-Proof.
-    intros HnormR.
-    generalize dependent Δ.
-    generalize dependent K.
-    induction HnormR; intros K' Δ Hwt; subst; auto.
-    - inversion Hwt; subst.
-
-      (* IHHnormR2:
-        K0 is the type of T2, which is K1
-      *)
-      specialize (IHHnormR2 K1 Δ H4).
-
-      (* IHHnormR1 K0 is the type of T1, which is K1 -> K'*)
-      specialize (IHHnormR1 (tp_arrow K1 K') Δ H2).
-
-            (* IHHnormR3:
-        K0 is the type of substituteTCA bX T2n T1n, hence it is the type of T1n
-        which should have the same type as T1.
-        Which is K1 -> K'.
-        *)
-      specialize (IHHnormR3 (tp_arrow K1 K') Δ).
-
-      admit.
-    - admit.
-    - 
-      (* specialize (IHHnormR ((bX, K)::Δ)). *)
-      inversion Hwt; subst.
-      specialize (IHHnormR K2 ((bX, K)::Δ) H4).
-      unfold normalizer.
-      destruct (strong_normalization_d Hwt). 
-       (* simpl. *)
-      unfold normalizer in IHHnormR.
-      destruct (strong_normalization_d H4) in IHHnormR.
-      simpl in IHHnormR.
-       
-      (* destruct IHHnormR. *)
-      destruct (step_d_f T0) eqn:Heq.
-      
-      
-      (*
-        Suppose (step_d_f T0 = None)
-        Then normalise T0 T0 and T0n = T0.
-
-        Then also in the goal, we have that the match becomes a None, so that it becomse
-        tmlam bX K T0.
-      *)
-       
-      
-      unfold step_d_f.
-      
-      admit.
-    - unfold normalizer.
-      destruct (strong_normalization_d Hwt).
-      simpl.
-      reflexivity.  
 Admitted.
 
 Theorem norm_sound Δ T (t tn : term) (Hwt : SN_STLC_named.has_type Δ t T) :
     normalizer Hwt = tn -> normalise t tn.
 Proof.
+  intros Hnorm.
+  unfold normalizer in Hnorm.
+
+  inversion Hnorm.
+  
 Admitted.
